Here are some basic integral formulas that are essential in calculus:

1. **Power Rule for Integration**:
   $$\int x^n \, dx = \frac{x^{n+1}}{n+1} + C \quad \text{(for } n \neq -1\text{)}$$

2. **Integral of a Constant**:
   $$
   \int a \, dx = ax + C
   $$

3. **Sum Rule**:
   $$
   \int (f(x) + g(x)) \, dx = \int f(x) \, dx + \int g(x) \, dx
   $$

4. **Difference Rule**:
   $$
   \int (f(x) - g(x)) \, dx = \int f(x) \, dx - \int g(x) \, dx
   $$

5. **Constant Multiple Rule**:
   $$
   \int a \cdot f(x) \, dx = a \int f(x) \, dx
   $$

6. **Integral of Exponential Functions**:
   $$
   \int e^x \, dx = e^x + C
   $$
   $$
   \int a^x \, dx = \frac{a^x}{\ln(a)} + C \quad \text{(for } a > 0 \text{ and } a \neq 1\text{)}
   $$

7. **Integral of Trigonometric Functions**:
   $$
   \int \sin(x) \, dx = -\cos(x) + C
   $$
   $$
   \int \cos(x) \, dx = \sin(x) + C
   $$
   $$
   \int \sec^2(x) \, dx = \tan(x) + C
   $$
   $$
   \int \csc^2(x) \, dx = -\cot(x) + C
   $$
   $$
   \int \sec(x) \tan(x) \, dx = \sec(x) + C
   $$
   $$
   \int \csc(x) \cot(x) \, dx = -\csc(x) + C
   $$

8. **Integral of Hyperbolic Functions**:
   $$
   \int \sinh(x) \, dx = \cosh(x) + C
   $$
   $$
   \int \cosh(x) \, dx = \sinh(x) + C
   $$

9. **Integral of the Natural Logarithm**:
   $$
   \int \ln(x) \, dx = x \ln(x) - x + C
   $$

These formulas form the foundation for solving a wide variety of integral problems.
#### Monash version
- $\int 1ğ‘‘ğ‘¥=ğ‘¥+ğ¶$
- $\int ğ‘ğ‘‘ğ‘¥=ğ‘ğ‘¥+ğ¶$
- $\int ğ‘¥ğ‘›ğ‘‘ğ‘¥=((ğ‘¥ğ‘›+1)/(ğ‘›+1))+ğ¶;ğ‘›â‰ 1$
- $\int sin(ğ‘¥)ğ‘‘ğ‘¥=âˆ’cos(ğ‘¥)+ğ¶$
- $\int cos(ğ‘¥)ğ‘‘ğ‘¥=sin(ğ‘¥)+ğ¶$
- $\int sec^2(ğ‘¥)ğ‘‘ğ‘¥=tan(ğ‘¥)+ğ¶$
- $\int csc^2(ğ‘¥)ğ‘‘ğ‘¥=âˆ’cot(ğ‘¥)+ğ¶$
- $\int sec(ğ‘¥(tan(ğ‘¥))ğ‘‘ğ‘¥=secğ‘¥+ğ¶$
- $\int cscğ‘¥(cotğ‘¥)ğ‘‘ğ‘¥=âˆ’cscğ‘¥+ğ¶$
- $\int (1/ğ‘¥)ğ‘‘ğ‘¥=ln|ğ‘¥|+ğ¶$
- $\int ğ‘’ğ‘¥ğ‘‘ğ‘¥=ğ‘’ğ‘¥+ğ¶$
- $\int ğ‘ğ‘¥ğ‘‘ğ‘¥=(ğ‘ğ‘¥/lnğ‘)+ğ¶;ğ‘>0,ğ‘â‰ 1$

Sum Rule of Integration:Â $\int(ğ‘“+ğ‘”)ğ‘‘ğ‘¥=\intğ‘“ğ‘‘ğ‘¥+\intğ‘”ğ‘‘ğ‘¥$

Difference Rule of Integration:Â $\int (ğ‘“âˆ’ğ‘”)ğ‘‘ğ‘¥=\int ğ‘“ğ‘‘ğ‘¥âˆ’\int ğ‘”ğ‘‘ğ‘¥$

Multiplication by ConstantÂ $\int ğ‘ğ‘“(ğ‘¥)ğ‘‘ğ‘¥=ğ‘\int ğ‘“(ğ‘¥)ğ‘‘ğ‘¥$.