*Not to be confused with [[Chain Rule (Probability)]]*


If$f(x) = g(h(x))$, then$f'(x) = g'(h(x)) \cdot h'(x)$.

alternatively
$ğ‘¦=ğ‘“(ğ‘¢)$Â andÂ $ğ‘¢=ğ‘”(ğ‘¥)$

i.e.Â $ğ‘¦=ğ‘“(ğ‘”(ğ‘¥))$

$$\frac{ğ‘‘}{ğ‘‘ğ‘¥}[ğ‘“(ğ‘”(ğ‘¥))]=ğ‘“'(ğ‘”(ğ‘¥))ğ‘”'(ğ‘¥)$$
**Chain Rule extended**
   - IfÂ $ğ‘¦=ğ‘“(ğ‘”(â„(ğ‘¥)))$:

$$\frac{ğ‘‘}{ğ‘‘ğ‘¥}[ğ‘“(ğ‘”(â„(ğ‘¥)))]=ğ‘“â€²(ğ‘”(â„(ğ‘¥)))ğ‘”â€²(â„(ğ‘¥))â„â€²(ğ‘¥)$$

### Partial

**Chain Rule with two independent variables**
   - $ğ‘¥=ğ‘”(ğ‘¢,ğ‘£)$ andÂ $ğ‘¦=â„(ğ‘¢,ğ‘£)$Â andÂ $ğ‘§=ğ‘“(ğ‘¥,ğ‘¦)$
   - i.e.Â $ğ‘§=ğ‘“(ğ‘”(ğ‘¢,ğ‘£),â„(ğ‘¢,ğ‘£))$

$$\frac{âˆ‚ğ‘§}{âˆ‚ğ‘¢}=\frac{âˆ‚ğ‘§}{âˆ‚ğ‘¥}\frac{âˆ‚ğ‘¥}{âˆ‚ğ‘¢}+\frac{âˆ‚ğ‘§}{âˆ‚ğ‘¦}\frac{âˆ‚ğ‘¦}{âˆ‚ğ‘¢}$$

- and

$$\frac{âˆ‚ğ‘§}{âˆ‚ğ‘£}=\frac{âˆ‚ğ‘§}{âˆ‚ğ‘¥}\frac{âˆ‚ğ‘¥}{âˆ‚ğ‘£}+\frac{âˆ‚ğ‘§}{âˆ‚ğ‘¦}\frac{âˆ‚ğ‘¦}{âˆ‚ğ‘£}$$